proofs/Prelude.v
@@ -50,8 +50,8 @@ Definition strong_last {A : Type} : forall ls : list A, ls <> [] -> A.
 Defined.
 
 Definition strong_nth :
-  forall {A : Set} (ls : list A) (idx : nat), idx < length ls -> A.
-  refine (fix f {A : Set} (ls : list A) (idx : nat) :=
+  forall {A : Set} (idx : nat) (ls : list A), idx < length ls -> A.
+  refine (fix f {A : Set} (idx : nat) (ls : list A) :=
               match idx, ls with
               | 0   , []       => fun pf => _
               | S m , []       => fun pf => _
@@ -63,3 +63,71 @@ Definition strong_nth :
   (* S m , [] *)
   + simpl in pf. omega.
 Defined.
+
+Lemma skipn_nil : forall A m, skipn m (@nil A) = (@nil A).
+Proof.
+  intros. induction m.
+  + reflexivity.
+  + reflexivity.
+Qed.
+
+Lemma skipn_cons :
+  forall {A : Set} (m : nat) (xs : list A) (x : A),
+  length (skipn m (x :: xs)) = length (skipn m xs) + 1.
+Proof.
+  intros. induction m.
+  + simpl. omega.
+  + simpl. Admitted.
+(* Qed. *)
+
+Lemma length_not_empty_inv {A B : Set} :
+  forall (xs : list A) (ys : list B),
+  length xs = length ys -> xs <> [] -> ys <> [].
+Proof. Admitted.
+
+(*
+
+Lemma length_not_zero_inv {A : Set} :
+  forall (xs : list A),  length xs <> 0 -> xs <> [].
+Proof.
+  intros. induction xs.
+  + unfold length in H. congruence.
+  + apply (cons_not_empty a xs).
+Qed.
+
+Lemma length_zero_inv {A : Set} :
+  forall (xs : list A),  length xs = 0 -> xs = [].
+Proof.
+  intros. induction xs.
+  + reflexivity.
+  + apply length_zero_iff_nil. apply H.
+Qed.
+
+Lemma length_not_zero_inv_inv {A : Set} :
+  forall (xs : list A), xs <> [] -> length xs <> 0.
+Proof.
+  intros. induction xs.
+  + congruence.
+  + unfold length. apply Nat.neq_succ_0.
+Qed.
+
+*)
+
+Lemma skipn_length : forall {A : Set}
+  (ls : list A) (n : nat), length (skipn n ls) = length ls - n.
+Proof.
+  intros. induction ls.
+  + simpl. rewrite skipn_nil. reflexivity.
+  + rewrite skipn_cons.
+Admitted.
+
+Lemma skipn_not_nil : forall {A : Set}
+  (ls : list A) (n : nat), n < length ls -> ls <> [] -> skipn n ls <> [].
+Proof. Admitted.
+
+Lemma min_eq : forall n, min n n = n.
+Proof.
+  intros. induction n.
+  + simpl. reflexivity.
+  + simpl. rewrite IHn. reflexivity.
+Qed.
